#+TITLE: Intro To Proofs Notes
#+AUTHOR: Denver Ellis

* Learning Objectives
1. How to find the inverse of a relation
2. How to find the composition of two relations.

* Inverse of a Relation
*** Definition
Let R be a relation from A to B. (Recall that this means R is a subset of AxB). The inverse of R, denoted by R^-1 is the set:

#+BEGIN_SRC latex
\begin{addmargin}[2em]{1em}
$R^-1 = \{(y, x): (x, y) \epsilon R\}$.
\end{addmargin}
#+END_SRC

Literally, given a relation R to find R^-1 we just swap the roles of x and y.

*** Example 1:
Consider the relation R = {(1, b), (1, c), (2, c)}. The inverse relation is R^-1 = {(b, 1), (c, 1), (c, 2)}.

For any set A, the inverse relation of I_A = {(a, a): a \epsilon A} is I_A.

The inverse relation of "less-than," R = {(x, y): x < y} is the "greater than" R^-1 = {(x, y): y < x}.

If a digraph is used to define/visualize a relation, the switching the direction of the arrows defines the inverse relation. Suppose that part of the digraph for some relation is

[[./imgs/img1.PNG]]

Then the inverse relation would include

[[./imgs/img2.PNG]]

in its digraph.

*** Example 2:
Let T = {(x, y) \epsilon \real x \real: y < 4x^2 - 7}. Find the inverse of T.

_Sketch of proof_:

(x, y) \epsilon T^-1 <=> (y, x) \epsilon T
            <=> x \lt 4y^2 - 7
            <=> x + 7 \lt 4y^2
            <=> 4y^2 \gt x + 7
            <=> y^2 \gt \frac{x+7}{4}
            <=> y \gt 1/2 * \radic(x + 7)

Thus T^-1 = {(x, y) \epsilon \real x \real: y \gt 1/2 \radic(x+7)}.

** Theorem 3.1.1:
Let R be a relation from A to B, Then

1) Dom(R^-1) = Rng(R).
2) Rng(R^-1) = Dom(R).

*** Proof:
1. The element b \epsilon Dom(R^-1) iff there exists an a \epsilon A such that (b, a) \epsilon R^-1. We have (b, a) \epsilon R^-1 iff (a, b) \epsilon R. Finally (a, b) \epsilon R iff b \epsilon Rng(R). Thus Dom(R^-1) = Rng(R).
2. The proof is similar. \qed

*** Definition
Let R be a relation from A to B and let s be a relation from B to C. The _composite_ or R and S, denoted by S \circ R, is the relation from A to C given by:

S \circ R = {(a, c): There exists a b\epsilon B such that (a, b) \epsilon R _and_ (b, c) \epsilon S}.

Note: S \circ R \sube A x C and while Dom(S \circ R) \sube Dom(R) it is not always true that Dom(S \circ R) = Dom(R).

*** Example 3:
Let A = {1, 2, 3, 4, 5}, B = {p, q, r, s, t}, and C = {x, y, z, w}. Let R be the relation from A to B

R = {(1, p), (1, q), (2, q), (3, r), (4, s)}

and let S be the relation from B to A

S = {(p, x), (q, x), (q, y), (s, z), (t, z)}.

Find S \circ R.

**** Solution:
We will use an arrow diagram to find S \circ R.

[[./imgs/img3.PNG]]

S \circ R = {(1, x), (1, y), (2, x), (2, y), (4, z)}. \qedsymbol

suppose that R is a relation from A to B and S is a relation from B to A. In general

S \circ R \ne R \circ S
A->A.   B->B.

*** Example 4:
Let R = {(x, y) \epsilon \real x \real: y = x + 1} and S = {(x, y): y = x^2}. Find S \circ R and R \circ S.

**** Solution
R \circ S = {(x, y): For some z \epsilon \real, (x, z) \epsilon S and (z, y) \epsilon R}
      = {(x, y): For some z \epsilon \real, z = x^2 and y = z + 1}
      = {(x, y): y = x^2 + 1}.

S \circ R = {(x, y): For some z \epsilon \real, (x, z) \epsilon R and (z, y) \epsilon S}
      = {(x, y): For some z \epsilon \real, z = x^2 and y = z + 1}
      = {(x, y): y = x^2 + 1}. \qedsymbol
** Theorem 3.1.2:
Let A, B, C and D be sets. Let R be a relation from A to B, S be a relation from B to C, and T be a relation from C to D. Then

1. (R^-1)^-1 = R
2. T \circ (S \circ R) = (T \circ S) \circ R
3. I_B \circ R = R \circ I_A = R
4. (S \circ R)^-1 = R^-1 \circ S^-1.
